Provide an inductive definition for HyperTr

eval/Evaluation.v
@@ -39,7 +39,6 @@ Section eval.
   Definition State := Var -> Val.
 
   Parameter Val_dec : EqDec Val eq.
-  Parameter Tag_dec : EqDec Tag eq.
   Parameter State_dec : EqDec State eq.
 
   Global Existing Instance Val_dec.
@@ -71,7 +70,6 @@ Section eval.
   Next Obligation.
     intros.
     destruct x as [[p i] s], y as [[q j] r].
-    
     destruct ((p, i, s) == (q, j, r)); firstorder.
   Qed.
   Definition Conf_dec := conf_eq_eqdec.
@@ -117,13 +115,31 @@ Section eval.
        | _ => None
        end.
 
-  Definition sem_step l k := option_chain eff (hd_error l) = Some k.
+  Definition sem_step l k
+    := option_chain eff (hd_error l) = Some k.
 
-  Inductive Tr : list Conf -> Prop :=
-  | Init : forall s, Tr [(root, start_tag, s)]
-  | Step : forall l (k : Conf), Tr l -> sem_step l k -> Tr (k :: l).
+  Inductive Tr (S : State -> Prop) : list Conf -> Prop :=
+  | Init : forall s, S s -> Tr S [(root, start_tag, s)]
+  | Step : forall l (k : Conf), Tr S l -> sem_step l k -> Tr S (k :: l).
 
   Definition EPath := Path eval_edge.
+
+  (* this is a simplicification, as we don't use particular sets of initial states *)
+(*  Inductive HyperTr (Σ : (State -> Prop) -> Prop) : (list Conf -> Prop) -> Prop :=
+  | HyperInit : forall S, Σ S -> HyperTr Σ (fun l => exists s, S s -> l = [(root, start_tag, s)])
+  | HyperStep : forall L (k : Conf), HyperTr Σ L -> HyperTr Σ (Tr (fun _ => False)).*)
+  Inductive HyperTr (Σ : (State -> Prop) -> Prop) : (list Conf -> Prop) -> Prop :=
+  | HyperInit : forall S, Σ S -> HyperTr Σ (fun l => exists s, S s -> l = [(root, start_tag, s)])
+  | HyperStep : forall L l (k : Conf), HyperTr Σ L -> L l -> sem_step l k -> HyperTr Σ (fun l' => l = l' \/ L l).
+
+  (* alternatively: *)
+  Definition Tr' (S : State -> Prop) : list Conf -> Prop
+    := fun t => exists s c, S s /\ EPath (root,start_tag,s) c t.
+
+  (* but hypertraces cannot be encoded in this way, because Paths are predicates on lists, 
+     while hypertraces operate on sets of traces *)
+
+  (* EVERYTHING beyound this point must be redone *)
 
   Hint Unfold Conf Coord.
   
@@ -134,62 +150,39 @@ Section eval.
     remember (p,i,s) as pis_c. revert p i s Heqpis_c.
     induction H; intros p i s Heqpis_c; [rewrite Heqstart_c|];econstructor;destruct b as [[b1 b2] b3].
     - eapply IHPath; eauto.
-    - subst c. destruct π;[inversion H|].
-      unfold sem_step;cbn.
-      path_simpl' H.
-      unfold eval_edge in H0. clear - H0.
-      unfold Coord in *.
-      destruct (eff (b1,b2,b3)).
-      + subst. reflexivity.
-      + contradiction.
+    - erewrite path_front; eauto. unfold eval_edge in H0.
+      unfold Conf,Coord in *.
+      destruct (eff (b1,b2,b3)); [subst c; eauto|congruence].
+      conv_bool. rewrite H0. reflexivity. 
   Qed.
-  
+
   Lemma Tr_EPath p i s π :
-    Tr π ->  hd_error π = Some (p,i,s) -> exists s0, EPath (root,start_tag,s0) (p,i,s) π.
+    Tr π ->  ne_front π = (p,i,s) -> exists s0, EPath (root,start_tag,s0) (p,i,s) π.
   Proof.
-    intros HTr Hfront.
+    intros HTr Hfront. exists (snd (ne_back π)).
     revert p i s Hfront. dependent induction HTr; cbn; intros p i s' Hfront.
-    - inversion Hfront. subst p i s'. eexists;econstructor.
-    - inversion Hfront. subst k.
-      remember (hd_error l) as c.
-      destruct c.
-      + destruct c as [[q j] r].
-        specialize (IHHTr q j r). exploit IHHTr.
-        destructH. eexists;econstructor;eauto.
-        unfold eval_edge.
-        unfold sem_step in H.
-        destruct l;cbn in H;[congruence|]. unfold EPath in IHHTr. path_simpl' IHHTr.
-        destruct (eff (q,j,r)).
-        * inversion H;eauto.
-        * congruence.
-      + unfold sem_step in H. destruct l;cbn in *;congruence.
-  Qed.
-  
-  Lemma eval_edge_tcfg_edge p q i j s r
-        (Heval : eval_edge (q,j,r) (p,i,s))
-    : tcfg_edge (q,j) (p,i).
-  Proof.
-    unfold eval_edge in Heval.
-    split.
-    - destruct (eff (q,j,r)) eqn:E;[|contradiction].
-      eapply step_conf_implies_edge. subst c;eauto.
-    - unfold eff in Heval.
-      destruct (eff' (q,r)).
-      destruct p0.
-      + inversion Heval;subst;auto.
-      + contradiction.
+    - cbn in *. rewrite <-Hfront; econstructor.
+    - rewrite <-Hfront.
+      econstructor; [eapply IHHTr; eauto|].
+      + repeat rewrite <-surjective_pairing. reflexivity.
+      + unfold eval_edge. do 2 erewrite <-surjective_pairing.
+        destruct (eff _); inversion H. apply beq_true. reflexivity.
   Qed.
 
   Lemma EPath_TPath k k' π :
-    EPath k k' π -> TPath (fst k) (fst k') (map fst π).
+    EPath k k' π -> TPath (fst k) (fst k') (ne_map fst π).
   Proof.
     intros H. dependent induction H; [|destruct c]; econstructor.
     - apply IHPath.
-    - cbn. destruct b. cbn. destruct c0, c. eapply eval_edge_tcfg_edge;eauto.
+    - unfold eval_edge in H0. unfold tcfg_edge,tcfg_edge'. repeat destr_let.
+      destruct (eff _) eqn:E; conv_bool; [|congruence]. split.
+      + rewrite H0 in E. eapply step_conf_implies_edge; eauto.
+      + unfold eff in E. destruct (eff' _) eqn:E'; [|congruence]. destruct p. destruct c,c.
+        inversion E. inversion H0. subst. reflexivity.
   Qed.
 
   Lemma EPath_TPath' k k' c c' π ϕ :
-    EPath k k' π -> c = fst k -> c' = fst k' -> ϕ = map fst π -> TPath c c' ϕ.
+    EPath k k' π -> c = fst k -> c' = fst k' -> ϕ = ne_map fst π -> TPath c c' ϕ.
   Proof.
     intros. eapply EPath_TPath in H;subst; eauto.
   Qed.
@@ -218,16 +211,21 @@ Section eval.
 
   (* This is the concrete transformer for sets of traces *)
   Definition sem_trace (ts : Traces) : Traces :=
-    fun tr' => exists tr k', ts tr /\ `tr' = (k' :: `tr).
+    fun tr' => exists tr k', ts tr /\ `tr' = (k' :<: `tr).
 
   (* This is the hypertrace transformer.
      Essentially, it lifts the trace set transformers to set of trace sets *)
   Definition sem_hyper (T : Hyper) : Hyper :=
     fun ts' => exists ts, T ts /\ ts' = sem_trace ts.
 
-  (* possibly unused
+  Lemma ne_hd_hd {A : Type} (a : A) l : a = ne_front l -> Some a = hd_error l.
+  Proof.
+    intros H.
+    induction l; cbn in *; subst a; reflexivity.
+  Qed.
+
   Lemma in_succ_in k p q t :
-    Tr (k :: t) -> In p t -> eff p = Some q -> In q (k :: t).
+    Tr (nlcons k t) -> In p t -> eff p = Some q -> In q (k :: t).
   Proof.
     intros. 
     revert dependent k. 
@@ -236,58 +234,41 @@ Section eval.
       * rewrite H5 in H1. inversion H1. left. reflexivity.
       * right. eapply IHt;eauto.
   Qed.
-   *)
 
-  Lemma Tr_eff_Some c k t
-        (Htr : Tr (c :: k :: t))
-    : eff k = Some c.
-  Proof.
-    inversion Htr.
-    unfold sem_step in H2. cbn in H2. eauto.
-  Qed.
-  
   Lemma in_pred_exists p i s k t :
-    (p,i,s) ∈ (k :: t) ->
+    In (p,i,s) (k :<: t) ->
     p <> root ->
-    Tr (k :: t) ->
-    exists q j r, (q, j, r) ∈ t /\ eff (q, j, r) = Some (p, i, s).
+    Tr (k :<: t) ->
+    exists q j r, In (q, j, r) t /\ eff (q, j, r) = Some (p, i, s).
   Proof.
     revert k.
     dependent induction t; intros k Hin Hneq Htr; inversion Htr.
-    - exfalso.
-      destruct Hin;[|contradiction].
-      subst k. inversion H0. eapply Hneq. rewrite H1. reflexivity.
-    - inversion H1. 
-    - subst.
-      destruct Hin.
-      + subst k.
-        destruct a as [[q j] r].
-        exists q, j, r. split;[left;auto|].
-        eapply Tr_eff_Some;eauto.
-      + specialize (IHt a).
-        exploit IHt.
-        destructH. do 3 eexists;eauto.
+    - destruct Hin; subst.
+      + destruct a as [[q j] r]. exists q,j,r.
+        split; cbn; eauto.
+      + exfalso. eapply Hneq. inversion H1.
+        destruct a,p0. cbn in H3. destruct H3;[|contradiction].
+        inversion H0;inversion H. subst p e. reflexivity.
+    - destruct Hin; subst.
+      + destruct a as [[q j] r].
+        exists q, j, r. split; [ constructor | assumption ]. reflexivity.
+      + edestruct IHt as [q [j [r [Hinq Hstep]]]]; try eassumption.
+        exists q, j, r. 
+        split; eauto.
+        cbn. tauto.
   Qed.
-  
+
   Lemma ivec_fresh : forall p i s (t : trace),
-      sem_step (`t) (p, i, s) -> forall j r, In (p, j, r) (`t) -> j <> i.
+      eff (ne_front (`t)) = Some (p, i, s) -> forall j r, In (p, j, r) (`t) -> j <> i.
   Proof.
     intros.
     destruct t; cbn in *.
-    remember (hd_error x) as c. destruct c.
-    - destruct c,c. eapply eff_tag_fresh.
-      + eapply Tr_EPath in t;eauto. destruct t as [s1 t].
-        eapply EPath_TPath in t; eauto.
-      + destruct x;cbn in Heqc;[congruence|].
-        inversion Heqc. subst c.
-        unfold sem_step in H. cbn in H.
-        destruct (eff' (e,s0)).
-        * destruct p0. inversion H. subst. eauto.
-        * congruence.
-      + eapply in_map with (f:=fst) in H0. eauto.
-    - destruct x.
-      + inversion t.
-      + cbn in Heqc. congruence.
+    remember (ne_front x) as c. destruct c,c. 
+    eapply eff_tag_fresh.
+    - eapply Tr_EPath in t;eauto. destruct t as [s1 t].
+      eapply EPath_TPath in t; eauto.
+    - eapply eff_eff_tag; eauto.
+    - eapply ne_map_in with (f:=fst) in H0. eauto.
   Qed.
   
   Lemma ivec_det : forall q j r r' p i i' s s',
@@ -340,8 +321,8 @@ Section eval.
   Qed.
 
   Lemma precedes_step_inv :
-    forall k t p s, Precedes' (k :: t) p s ->
-               Tr (k :: t) ->
+    forall k t p s, Precedes' (nlcons k t) p s ->
+               Tr (nlcons k t) ->
                lab_of p <> lab_of s ->
                In p t.
   Proof.
@@ -350,13 +331,13 @@ Section eval.
     inv_tr Hprec.
     - firstorder.
     - eapply precedes_in in H5.
-      eapply prefix_cons_cons in Hpre.      
+      rewrite <-nlcons_to_list in Hpre. eapply prefix_cons_cons in Hpre.      
       eapply in_prefix_in; eauto.
   Qed.
 
   Lemma in_exists_pred p i s k (t : trace) :
-    In (p, i, s) (k :: `t) ->
-    sem_step (`t) k ->
+    In (p, i, s) (k :<: `t) ->
+    eff (ne_front (`t)) = Some k ->
     p <> root ->
     exists q j r, In (q, j, r) (`t) /\ eff (q, j, r) = Some (p, i, s).
   Proof.
@@ -365,20 +346,14 @@ Section eval.
     destruct H; [subst k| revert dependent k];
       dependent induction l; inversion tr; subst; intros. 
     - exists root, start_tag, s0. split; [ constructor | eauto ]; eauto.
-    - cbn in Heff, H2. destruct a as [[q j] r]. exists q,j,r. firstorder. 
+    - cbn in Heff, H2. destruct a as [[q j] r]. exists q,j,r. firstorder. cbn. left; reflexivity.
     - exfalso. inversion H; inversion H0. subst p; contradiction.
     - destruct H.
-      + subst a. remember (hd_error l) as qjr. destruct qjr as [qjr|qjr].
-        2: destruct l; unfold sem_step in H3;cbn in *;congruence.
-        destruct qjr as [[q j] r].
-        exists q,j,r. split; [econstructor 2 | eauto].
-        * destruct l;[inversion H2|]. cbn in Heqqjr. inversion Heqqjr.
-          setoid_rewrite H0. left. auto.
-        * unfold sem_step in H3.
-          destruct l;[inversion H2|].
-          cbn in H3. cbn in Heqqjr. inversion Heqqjr. subst c. eauto.
+      + subst a. remember (ne_front l) as qjr. destruct qjr as [[q j] r].
+        exists q,j,r. split; [econstructor 2 | eauto]. setoid_rewrite Heqqjr.
+        clear; destruct l; cbn; eauto.
       + eapply IHl in H2; eauto. destruct H2 as [q [j [r [Hin Hstep]]]].
-        exists q, j, r. split; eauto. 
+        exists q, j, r. split; eauto. econstructor 2; eauto.
   Qed.
 
   Lemma root_prefix (t : trace) : exists s, Prefix ((root, start_tag, s) :: nil) (`t).
@@ -396,27 +371,25 @@ Section eval.
     destruct t as [l tr]. induction l; inversion tr; subst; cbn in *; intros i Hin.
     - destruct Hin as [Hin|Hin]; [inversion Hin; eauto|contradiction].
     - destruct Hin.
-      + exfalso. destruct l;[inversion H1|]. destruct c as [[q j] r].
+      + exfalso. destruct (ne_front l) as [[q j] r].
         eapply root_no_pred. subst a.
-        apply edge_spec. unfold is_effect_on. exists j,i,r,s.
-        eapply Tr_eff_Some;eauto.
+        apply edge_spec. unfold is_effect_on. exists j,i,r,s. eapply H2.
       + eapply IHl; eauto.
   Qed.
 
   Lemma trace_destr_in_in k k' (t : trace) :
     In k (`t) -> In k' (`t)
-    -> exists (t': trace), hd_error (`t') = Some k' /\ In k (`t') \/ hd_error (`t') = Some k /\ In k' (`t').
+    -> exists (t': trace), ne_front (`t') = k' /\ In k (`t') \/ ne_front (`t') = k /\ In k' (`t').
   Proof.
     intros Hin Hin'.
     destruct t as [t tr]. cbn in *.
     induction t; inversion tr; cbn in *.
-    - subst t. destruct Hin; [|contradiction]; destruct Hin'; [|contradiction].
-      subst a k.
-      exists (exist _ [k'] tr). cbn. tauto.
+    - destruct Hin; [|contradiction]; destruct Hin'; [|contradiction].
+      exists (exist _ (ne_single a) tr). cbn. tauto.
     - destruct Hin, Hin'; [| | |eapply IHt; eauto]; subst.
-      + exists (exist _ (k' :: t) tr ). cbn. tauto.
-      + exists (exist _ (k :: t) tr). cbn. tauto.
-      + exists (exist _ (k' :: t) tr). cbn. tauto.
+      + exists (exist _ (k' :<: t) tr ). cbn. tauto.
+      + exists (exist _ (k :<: t) tr). cbn. tauto.
+      + exists (exist _ (k' :<: t) tr). cbn. tauto.
   Qed.
 
   Ltac trace_proj t :=
@@ -430,35 +403,50 @@ Section eval.
     intros His Hir. eapply trace_destr_in_in in His; eauto.
     destruct His as [[t' tr'] [[Hf Hin]|[Hf Hin]]]; cbn in *.
     - induction t'; inversion tr'.
-      + cbn in Hin,Hf. subst t'. destruct Hin; [|contradiction]. subst a. inversion Hf. reflexivity.
-      + subst. cbn in *. destruct a as [[q j] r']. inversion Hf. subst.
-        destruct Hin;  [inversion H; reflexivity|].
+      + cbn in Hin,Hf. destruct Hin; [|contradiction]. subst a. inversion H. reflexivity.
+      + cbn in *. subst. destruct Hin; [inversion H; reflexivity|].
         trace_proj t'.
         eapply ivec_fresh in H2; eauto. contradiction.
     - induction t'; inversion tr'.
-      + cbn in Hin,Hf. subst t'. destruct Hin; [|contradiction]. subst a. inversion Hf. reflexivity.
-      + cbn in *. subst. destruct a as [[q j] r']. inversion Hf. subst.
-        destruct Hin; [inversion H; reflexivity|].
+      + cbn in Hin,Hf. destruct Hin; [|contradiction]. subst a. inversion H. reflexivity.
+      + cbn in *. subst a. destruct Hin; [inversion H3; reflexivity|].
         trace_proj t'. eapply ivec_fresh in H2; eauto. contradiction.
   Qed.
 
-  Lemma prefix_trace (l l' : list Conf) c :
-    Prefix (c :: l) l' -> Tr l' -> Tr (c :: l).
+  Lemma prefix_trace (l l' : ne_list Conf) :
+    Prefix l l' -> Tr l' -> Tr l.
   Proof.
     intros Hpr Htr. induction Htr;cbn in *.
-    - inversion Hpr;[econstructor|]. inversion H1.
+    - inversion Hpr;[simpl_nl' H1;rewrite H1;econstructor|]. inversion H1.
+      simpl_nl' H5. contradiction.
     - inversion Hpr.
-      + subst. econstructor;eauto.
+      + rewrite nlcons_to_list in H2. simpl_nl' H2. rewrite H2. econstructor;eauto.
       + eapply IHHtr;eauto.
   Qed.
 
-  Lemma eval_det c0 c c' : eval_edge c0 c -> eval_edge c0 c' -> c = c'.
+  Lemma eval_det c0 c c' : eval_edge c0 c = true -> eval_edge c0 c' = true -> c = c'.
   Proof.
-    intros Hcc Hcc'. unfold eval_edge in *. destruct (eff c0); subst;auto. contradiction.
+    intros Hcc Hcc'. unfold eval_edge in *. destruct (eff c0); conv_bool;[|congruence].
+    rewrite <-Hcc, <-Hcc'. reflexivity.
   Qed.
 
-(*  Lemma tr_succ_eq (l : list Conf) (k k' : Conf) :
-    ne_back (k :: l) = ne_back (k' :: l) -> Tr (k :: l) -> Tr (k' :: l) -> k = k'.
+  Lemma necons_nlcons_inv {A : Type} (a a' : A) l l' :
+    (a :<: l) = a' :< l' -> a = a' /\ ne_to_list l = l'.
+  Proof.
+    intro H. split.
+    all:destruct l'; cbn in *; [congruence|].
+    1:revert a a' a0 l' H; induction l; intros b b' b0 l' H; cbn in *.
+    1,2: inversion H; split;eauto.
+    revert a a' a0 l' H; induction l; intros b b' b0 l' H; cbn in *.
+    - destruct l'; cbn in *;congruence.
+    - f_equal.
+      + inversion H. destruct l';inversion H2. reflexivity.
+      + destruct l'; cbn in *; inversion H; subst. eapply IHl.
+        reflexivity. Unshelve. eauto.
+  Qed.
+
+  Lemma tr_succ_eq (l : list Conf) (k k' : Conf) :
+    ne_back (k :< l) = ne_back (k' :< l) -> Tr (k :< l) -> Tr (k' :< l) -> k = k'.
   Proof.
     intros Hback Htr Htr'.
     inversion Htr; inversion Htr'; subst.
@@ -471,7 +459,7 @@ Section eval.
     apply ne_to_list_inj in H22. apply ne_to_list_inj in H02. rewrite H22 in H4. rewrite H02 in H1.
     simpl_nl' H1. simpl_nl' H4.
     eapply eval_det; unfold eval_edge; [rewrite H1|rewrite H4]; conv_bool; reflexivity.
-  Qed.*)
+  Qed.
   
   Lemma prefix_eff_cons_cons k k' l l' :
     (*    eff (ne_front l) = Some k
@@ -481,8 +469,8 @@ Section eval.
     -> Prefix (k :: l) (k' :: l').
      *)
     l <> nil
-    -> Tr (k :: l)
-    -> Tr (k' :: l')
+    -> Tr (k :< l)
+    -> Tr (k' :< l')
     -> Prefix l l'
     -> Prefix (k :: l) (k' :: l').
   Proof.
@@ -491,15 +479,7 @@ Section eval.
     induction Hpre; intros k' Htr'.
     - enough (k = k').
       + subst k'. econstructor.
-      + destruct k as [[q j] r]. destruct k' as [[q' j'] r'].
-        eapply Tr_EPath in Htr. 2: cbn;reflexivity.
-        eapply Tr_EPath in Htr'. 2: cbn;reflexivity.
-        do 2 destructH.
-        inversion Htr. 1: symmetry in H4;contradiction.
-        inversion Htr'. 1: symmetry in H9;contradiction.
-        subst. destruct l. 1: inversion H0.
-        path_simpl' H0. path_simpl' H5.
-        eapply eval_det;eauto.
+      + eapply tr_succ_eq; eauto. destruct l; cbn; eauto; contradiction.
     - econstructor. eapply IHHpre; eauto. inversion Htr'; eauto.
   Qed.
   
@@ -507,73 +487,74 @@ Section eval.
     Precedes' (`t) (q', j', r') (q, j, r) ->
     eff (q, j, r) = Some (p, i, s) ->
     p <> q' ->
-    Tr (k' :: (`t)) ->
-    Precedes' (k' :: (`t)) (q', j', r') (p, i, s).
+    Tr (k' :<: (`t)) ->
+    Precedes' (k' :<: (`t)) (q', j', r') (p, i, s).
   Proof.
     intros Hprec Heff Hneq Htr.
     destruct Hprec as [t' [Hpre Hprec]].
-    exists ((q,j,r) :: t').
+    exists (nlcons (q,j,r) t').
     split.
     - clear Hprec Hneq. 
       unfold Conf in Hpre. unfold Coord in Hpre.
       set (t2 := (q,j,r) :: t') in *.
       destruct t as [t tr]. unfold "`" in *. cbn. subst t2.
-      eapply prefix_eff_cons_cons; eauto;[congruence| eauto].
+      simpl_nl.
+      eapply prefix_eff_cons_cons; eauto;[congruence| |simpl_nl;eauto].
       cbn. econstructor.
       + eapply prefix_trace.
-        * eauto.
-        * inversion Htr; eauto. subst t. inversion Hpre. 
-      + eauto. 
+        * simpl_nl;eauto.
+        * inversion Htr; eauto.
+      + simpl_nl; eauto.
     - econstructor; cbn; eauto. 
+      rewrite <-nlcons_to_list. eauto.
   Qed.
        
-  (* possibly unused
+  
   Lemma precedes_step l q j r p i s :
-    forall k, (q, j, r) ∈ l ->
+    forall k, In (q, j, r) l ->
          p <> q ->
          eff (q, j, r) = Some (p, i, s) ->
-         Tr (k :: l) -> 
-         Precedes' (k :: l) (q, j, r) (p, i, s).
+         Tr (nlcons k l) -> 
+         Precedes' (nlcons k l) (q, j, r) (p, i, s).
   Proof.
     intros k Hin Hneq Heff Htr.
-    assert ((p,i,s) ∈ (k :: l)) as Hin'.
+    assert (In (p,i,s) (nlcons k l)) as Hin'.
     {
       revert dependent k.
       induction l; intros k Htr; cbn in Htr; inversion Htr; inversion Hin; cbn; subst.
-      - left. rewrite H2 in Heff. inversion Heff. reflexivity.
-      - right. cbn in IHl. eauto.
+      - left. rewrite nlcons_front in H2. rewrite H2 in Heff. inversion Heff. reflexivity.
+      - right. eauto.
     }
-    exists (prefix_nincl (p,i,s) (k :: l)). split.
+    exists (prefix_nincl (p,i,s) (nlcons k l)). split.
     - eapply prefix_nincl_prefix; eauto.
     - revert dependent k. induction l; intros k Htr Hin'; inversion Hin; inversion Hin'; subst.
       + cbn. destruct ((p,i,s) == (p,i,s)); [destruct e|exfalso; eapply c; reflexivity].
         econstructor; [cbn; eauto|]. destruct l; cbn; econstructor.
       + exfalso.
+        unfold nlcons in Htr. fold (nlcons (q,j,r) l) in Htr.
         inversion Htr; subst.
-        assert (k = (p,i,s)) as Hk.
-        { eapply Tr_eff_Some in Htr. rewrite Htr in Heff. inversion Heff. auto. }
-        subst k.
         eapply ivec_fresh.
-        * instantiate (4:=exist _ _ H2). unfold "`". eapply H3.
+        * rewrite <-Heff. instantiate (1:=exist _ _ H2). unfold "`". rewrite nlcons_front. reflexivity.
         * cbn. eauto.
         * reflexivity.
       + exfalso.
-        inversion Htr; subst.
-        destruct a as [[q' j'] r'].
+        unfold nlcons in Htr. fold (nlcons a l) in Htr.
+        inversion Htr; subst. 
         eapply ivec_fresh.
-        * instantiate (4:=exist _ _ H2). unfold "`". eauto.
-        * cbn. give_up.
+        * setoid_rewrite <-H3. instantiate (1:=exist _ _ H2). unfold "`". rewrite nlcons_front.
+          reflexivity.
+        * cbn; rewrite <-nlcons_to_list. eapply in_succ_in in H; eauto. 
         * reflexivity.
-      + cbn. destruct ((p,i,s) == k).
+      + unfold nlcons. fold (nlcons a l). cbn. destruct ((p,i,s) == k).
         * destruct e. exfalso.
           inversion Htr; subst.
           eapply ivec_fresh.
-          -- instantiate (4:=exist _ _ Htr). unfold "`". eauto. give_up.
+          -- setoid_rewrite <-H4. instantiate (1:=exist _ _ H3). unfold "`". rewrite nlcons_front.
+             reflexivity.
           -- cbn. eauto.
           -- reflexivity.
         * eapply IHl; eauto. cbn in Htr. inversion Htr; subst; eauto.
   Qed.
-  *)
 
   Lemma no_def_untouched :
     forall p q x, is_def x q p = false -> forall i j s r, eff (q, j, r) = Some (p, i, s) -> r x = s x.
@@ -609,71 +590,68 @@ Section eval.
    *)
   
   Lemma Tr_CPath l :
-    Tr l -> CPath root (fst (fst (hd (root,start_tag,zero) l))) (map fst (map fst l)).
+    Tr l -> CPath root (fst (fst (ne_front l))) (ne_map fst (ne_map fst l)).
   Proof.
-    intro H. destruct l;[inversion H|].
-    eapply Tr_EPath in H;[| repeat rewrite <-surjective_pairing; reflexivity].
+    intro H. eapply Tr_EPath in H;[| repeat rewrite <-surjective_pairing; reflexivity].
     destruct H as [s0 H]. cbn. 
     eapply EPath_TPath in H. cbn in H. eapply TPath_CPath in H. eauto.
   Qed.
 
-  Definition Tr' (l : list Conf) :=
+  Definition Tr' (l : ne_list Conf) :=
     exists l', Tr l' /\ Postfix l l'.
+  
 
-  Lemma tr_lc_lt p i s1 s2 l1 l2 q1 q2 j1 j2 r1 r2
-        (Htr1 : Tr ((p, i, s1) :: (q1,j1,r1) :: l1))
-        (Htr2 : Tr ((p, i, s2) :: (q2,j2,r2) :: l2))
-    : exists brk,
-      last_common ((q1,j1) :: map fst l1) ((q2,j2) :: map fst l2) (brk).
+  Definition EPath' π := EPath (ne_back π) (ne_front π) π.
+
+  Lemma epath_epath' r i0 s0 p i s t
+        (Hpath : EPath (r,i0,s0) (p,i,s) t)
+    : EPath' t.
   Proof.
-    inversion Htr1. subst k l.
-    inversion Htr2. subst k l.
-    eapply Tr_EPath in H1. 2:cbn;eauto.
-    eapply Tr_EPath in H3. 2:cbn;eauto.
-    do 2 destructH.
-    setoid_rewrite cons_rcons' in H1.
-    setoid_rewrite cons_rcons' in H3.
-    pose (l1' := (rev (tl (rev ((q1, j1, r1) :: l1))))).
-    pose (l2' := (rev (tl (rev ((q2, j2, r2) :: l2))))).
-    eapply path_back in H1 as Hback1. rewrite <-Hback1 in *.
-    eapply path_back in H3 as Hback2. rewrite <-Hback2 in *.
-    specialize (ne_last_common (map fst l1') (map fst l2') (root,start_tag)) as Hlc.
-    destructH.
-    exists s.
-    enough ((q2,j2) :: map fst l2 = map fst l2' :r: (root,start_tag)).
-    enough ((q1,j1) :: map fst l1 = map fst l1' :r: (root,start_tag)).
-    * rewrite H. rewrite H0. eauto.
-    * clear - Hback1. subst l1'.
-      fold (fst (root,start_tag,s3)). 
-      rewrite <-map_rcons.
-      rewrite Hback1.
-      rewrite <-cons_rcons'. cbn. eauto.
-    * clear - Hback2. subst l2'.
-      fold (fst (root,start_tag,s0)).
-      rewrite <-map_rcons.
-      rewrite Hback2.
-      rewrite <-cons_rcons'. cbn. eauto.
+    unfold EPath'. eapply path_back in Hpath as Hback.
+    eapply path_front in Hpath as Hfront.
+    rewrite Hfront,Hback. assumption.
+  Qed.
+
+  
+  Lemma ne_back_trace t :
+    Tr t -> exists s, ne_back t = (root,start_tag,s).
+  Proof.
+    intro Htr.
+    induction Htr; firstorder. exists s. cbn; reflexivity.
+  Qed.
+
+  Lemma tr_lc_lt' p i s1 s2 l1 l2
+        (Htr1 : Tr ((p, i, s1) :<: l1))
+        (Htr2 : Tr ((p, i, s2) :<: l2))
+    : exists brk,
+      last_common (ne_map fst l1) (ne_map fst l2) (brk).
+  Proof.
+    eapply ne_last_common. repeat rewrite ne_back_map.
+    eapply ne_back_trace in Htr1 as [s1' Htr1]. cbn in Htr1.
+    eapply ne_back_trace in Htr2 as [s2' Htr2]. cbn in Htr2.
+    setoid_rewrite Htr1. setoid_rewrite Htr2. cbn;eauto.
+  Qed.
+
+  Lemma tr_lc_lt p i s1 s2 q1 q2 j1 j2 r1 r2 l1 l2
+        (Htr1 : Tr ((p, i, s1) :<: (q1, j1, r1) :< l1))
+        (Htr2 : Tr ((p, i, s2) :<: (q2, j2, r2) :< l2))
+    : exists br k,
+      last_common ((q1, j1) :: map fst l1) ((q2, j2) :: map fst l2) (br,k).
+  Proof.
+    enough (exists brk,
+               last_common (ne_map fst ((q1, j1, r1) :< l1)) (ne_map fst ((q2, j2, r2) :< l2)) brk).
+    { (simpl_nl' H;cbn in H;destruct H as [[br k] H];eauto). }
+    eapply tr_lc_lt';eauto.
   Qed.
 
   Lemma tr_tpath_cons2 p i s q j r l
-        (Htr : Tr ((p,i,s) :: (q,j,r) :: l))
-    : TPath (root,start_tag) (p,i) ((p, i) :: (q, j) :: map fst l).
+        (Htr : Tr ((p,i,s) :<: (q,j,r) :< l))
+    : TPath' ((p, i) :<: (q, j) :< map fst l).
   Proof.
     eapply Tr_EPath in Htr as Htr; cbn;eauto. destruct Htr as [s01 Htr].
     eapply EPath_TPath in Htr.
-    cbn in *. auto.
-  Qed.
-
-  Lemma Tr_NoDup l
-        (Htr : Tr l)
-    : NoDup (map fst l).
-  Proof.
-    destruct l;[inversion Htr|].
-    destruct c as [[q j] r]. cbn.
-    eapply Tr_EPath in Htr;[|cbn;reflexivity].
-    destructH.
-    eapply EPath_TPath in Htr. cbn in Htr.
-    eapply tpath_NoDup;eauto.
+    cbn in *. unfold TPath'. simpl_nl' Htr. cbn in *.
+    eapply path_back in Htr as Hback. cbn in Hback. unfold Coord in *. rewrite Hback;eauto.
   Qed.
 
   Lemma tr_lift_succ l q q' j j'
@@ -687,55 +665,57 @@ Section eval.
     - revert dependent l1. revert q q' j j'. induction l;intros.
       + cbn in *. congruence.
       + cbn in *. inversion Hpath;subst.
-        1:cbn in Hsucc; congruence. 
         exploit' IHl. destruct l1.
         * destruct a. inversion H1;subst;cbn in Hsucc; inversion Hsucc;[subst q j|].
           -- cbn in *. 
              exists s0, s, nil, nil. cbn. reflexivity.
-          -- exfalso. destruct l0; cbn in H6;[inversion H|congruence].
+          -- exfalso. destruct l0; cbn in H6; congruence.
         * destruct a. cbn in *. destruct c.
           specialize (IHl e q t j l1). inversion Hsucc;subst. exploit IHl. destructH.
           exists r', s, ((e,t,r) :: (tl (tl l))), nil. cbn.
           unfold succ_in in IHl. destructH.
           destruct l2;cycle 1.
-          { 
-            exfalso.
-            eapply Tr_NoDup in H1.
-            enough (fst c = (q,j)).
-            - rewrite IHl in H1. cbn in H1. rewrite H in H1.
-              rewrite map_app in H1. clear - H1.
-              inversion H1. eapply H2.
-              eapply in_or_app. right. auto.
-            - clear - IHl Hsucc.
-              inversion Hsucc. rewrite IHl in H0. cbn in H0.
-              inversion H0. reflexivity.
-          } 
+          { exfalso.
+            cbn in IHl. rewrite IHl in H3. cbn in H3.
+            inversion H3.
+            inversion H1;subst.
+            - destruct l2; cbn in IHl; congruence.
+            - destruct k. destruct c0. eapply Tr_EPath in H1. 2: cbn;reflexivity.
+              destructH. eapply EPath_TPath in H1. cbn in H1.
+              eapply tpath_NoDup in H1. cbn in H1. inversion H1. subst. apply H8.
+              clear - Hsucc IHl.
+              cbn in *. inversion Hsucc. subst. inversion IHl. subst.
+              rewrite <-to_list_ne_map. setoid_rewrite H1.
+              clear.
+              induction l2;cbn in *.
+              + left. auto.
+              + right. auto.
+          }
           assert (l1 = map fst l0).
           {
             cbn in IHl. clear - IHl H3.
-            rewrite IHl in H3. cbn in H3. inversion H3. reflexivity.
+            destruct l. 1: cbn in IHl; congruence.
+            cbn in IHl, H3. inversion IHl; inversion H3; subst.
+            destruct l;cbn in H4; inversion H4.
+            - cbn in H1. destruct l0; cbn in H1;[|congruence]. cbn. auto.
+            - cbn in IHl. inversion IHl. rewrite H7. reflexivity.
           } 
           rewrite H in H3. cbn in IHl.
           f_equal.
-          inversion H1.
+          inversion H1;subst.
           -- exfalso. cbn in *. congruence.
-          -- cbn in Hsucc,H2,H3. destruct k. cbn in Hsucc,H3.
-             rewrite <-H5 in IHl. 
-             inversion H0.
-             ++ cbn. destruct c. inversion IHl. subst. congruence.
-             ++ cbn. destruct c. inversion IHl. subst. f_equal. f_equal. inversion H13. auto.
+          -- cbn in Hsucc,H2,H3. destruct k. cbn in Hsucc,H3. inversion H0;subst.
+             ++ cbn. destruct c. inversion IHl. f_equal.
+             ++ cbn. destruct c. inversion IHl. f_equal.
     - destruct l; cbn.
       + exfalso. destruct l2;cbn in Hsucc; inversion Hsucc.
-      + cbn in Hsucc. inversion Hsucc.
-        destruct l. 1: cbn in H1;congruence'.
-        inversion Hpath;subst.
-        eapply IHl2 in H1;eauto.
-        destructH. do 2 eexists. eapply succ_cons. eauto.
+      + cbn in Hsucc. inversion Hsucc. inversion Hpath;subst.
+        eapply IHl2 in H1;eauto. destructH. do 2 eexists. eapply succ_cons. eauto.
   Qed.
   
   Lemma tr_succ_eff' p q q' br i j k s r r' r0 l
-        (Htr : Tr ((p, i, s) :: l))
-        (Hsucc : (q, j, r) ≻ (br, k, r0) | (p, i, s) :: l)
+        (Htr : Tr ((p, i, s) :< l))
+        (Hsucc : (q, j, r) ≻ (br, k, r0) | (p, i, s) :< l)
         (Heff : eff' (br,r0) = Some (q',r'))
     : q = q'.
   Proof.
@@ -744,11 +724,10 @@ Section eval.
     induction l2;intros.
     - cbn in Hsucc.
       destruct l. 1: cbn in *; congruence.
-      inversion Hsucc. subst.
-      eapply Tr_eff_Some in Htr.
-      unfold eff in Htr.
-      rewrite Heff in Htr.
-      inversion Htr. reflexivity.
+      cbn in *.  destruct p0. destruct p0. inversion Hsucc. subst. simpl_nl' H3. inversion H3.
+      subst. inversion Htr. subst. simpl_nl' H2.
+      unfold eff in H2. destruct (eff' (br, r0));[|congruence].
+      destruct p. inversion Heff. inversion H2. subst. auto.
     - cbn in Hsucc.
       destruct l. 1: cbn in *; destruct l2; cbn in Hsucc;congruence.
       destruct p0. destruct p0.
@@ -762,65 +741,48 @@ Section eval.
   Proof.
     exists nil, l. rewrite <-app_assoc. rewrite <-app_comm_cons. cbn. reflexivity.
   Qed.
-
-  Lemma succ_in_cons_eq (A : Type) (a b c : A) l
-        (Hsucc : a ≻ b | a :: c :: l)
-        (Hnd : NoDup (a :: c :: l))
-    : b = c.
-  Proof.
-    inversion Hnd. subst.
-(*    destruct (b == c);[auto|].*)
-    unfold succ_in in Hsucc. destructH.
-    destruct l2.
-    - cbn in *. inversion Hsucc. auto.
-    - exfalso.
-      eapply H1. cbn in Hsucc. inversion Hsucc;subst.
-      clear - H3. destruct l2;intros;inversion H3;subst;cbn in *;eauto.
-  Qed.
   
-  Lemma succ_in_cons_neq (A : Type) (a b c d : A) l
-        (Hsucc : a ≻ b | d :: c :: l)
-        (Hnd : NoDup (c :: l))
-        (Hneq : a <> d)
-    : a ≻ b | c :: l.
-  Proof.
-    unfold succ_in in Hsucc. destructH.
-    destruct l2.
-    - cbn in Hsucc. inversion Hsucc. subst. contradiction.
-    - cbn in Hsucc. inversion Hsucc. subst. eexists;eexists. eauto.
-  Qed.
-  
-  Lemma succ_in_tpath_eff_tag p q i j t a b
-        (Hpath : TPath a b t)
+  Lemma succ_in_tpath_eff_tag p q i j t
+        (Hpath : TPath' t)
         (Hsucc : (p,i) ≻ (q,j) | t)
     : eff_tag q p j = i.
   Proof.
-    induction Hpath.
+    induction t.
     - exfalso. unfold succ_in in Hsucc. destructH. cbn in Hsucc.
       destruct l2;cbn in Hsucc;try congruence. destruct l2; cbn in Hsucc; try congruence.
-    -
-      destruct π;[inversion Hpath|].
-      decide (c = (p,i)).
-      + subst c. eapply succ_in_cons_eq in Hsucc;eauto.
-        * path_simpl' Hpath. subst b. unfold tcfg_edge,tcfg_edge' in H. destruct H. auto.
-        * eapply tpath_NoDup. econstructor;eauto.
-      + eapply succ_in_cons_neq in Hsucc;eauto.
-        path_simpl' Hpath.
-        eapply tpath_NoDup. eauto.
+    - decide (a = (p,i)).
+      + unfold TPath' in Hpath. eapply tpath_NoDup in Hpath as Hnd.
+        cbn in Hnd. inversion Hnd. subst.
+        cbn in Hsucc.
+        unfold succ_in in Hsucc. destructH.
+        destruct l2;cycle 1.
+        { cbn in Hsucc. inversion Hsucc. rewrite H3 in H1. exfalso. eapply H1. clear.
+          induction l2;cbn;eauto.
+        }
+        cbn in Hsucc. cbn in Hpath.
+        inversion Hsucc. rewrite nlcons_to_list in H0. eapply ne_to_list_inj in H0.
+        rewrite H0 in Hpath. eapply tcfg_edge_spec.
+        inversion Hpath. path_simpl' H3. auto.
+      + eapply IHt.
+        * unfold TPath' in Hpath. cbn in Hpath. inversion Hpath. subst. destruct a.
+          destruct (ne_back t). inversion Hpath. destruct b0.
+          eapply tpath_tpath'; eauto.
+        * cbn in Hsucc. unfold succ_in in Hsucc. destructH.
+          destruct l2. 1: exfalso;cbn in Hsucc;inversion Hsucc;subst;contradiction.
+          cbn in Hsucc. inversion Hsucc. exists l1, l2;eauto.
   Qed.
   
   Lemma eff_tcfg p q i j s r
         (Heff : eff (p,i,s) = Some (q,j,r))
-    : tcfg_edge (p,i) (q,j).
+    : tcfg_edge (p,i) (q,j) = true.
   Proof.
     eapply eff_eff_tag in Heff as Heff'. unfold tcfg_edge, tcfg_edge'.
     eapply step_conf_implies_edge in Heff. conv_bool; firstorder.
   Qed.
 
-  (* possibly unused 
   Lemma tr_tpath_cons1 (l : list Conf) c
-        (Htr : Tr (c :: l))
-    : TPath (root,start_tag) (fst c) ((fst c) :: map fst l).
+        (Htr : Tr (c :< l))
+    : TPath' ((fst c) :< map fst l).
   Proof.
     revert dependent c.
     induction l; intros c Htr; inversion Htr; cbn; [econstructor|]. unfold TPath'. cbn.
@@ -829,7 +791,6 @@ Section eval.
     simpl_nl' H2. destruct a as [[p i] s]. destruct c as [[q j] r]. cbn. simpl_nl.
     eapply eff_tcfg;eauto.
   Qed.
-   *)
   
   Lemma prec_lab_prec_fst p i s l
         (Hprec : Precedes lab_of l (p,i,s))
@@ -853,26 +814,31 @@ Ltac spot_path_e :=
   let i := fresh "i" in
   let s := fresh "s" in
   lazymatch goal with 
-  | [ H : Tr ((?p,?i,?s) :: ?t) |- _ ] => eapply Tr_EPath in H;[|cbn;reflexivity]; destructH' H; cbn in H
-  | [ H : Tr ?t |- _ ] => destruct (hd_error t) as [[[p i] s]|N] eqn:Q;
-                        [eapply Tr_EPath in H;[clear Q|apply Q]; destructH' H; cbn in H
-                        |inversion H]
+  | [ H : Tr ((?p,?i,?s) :<: ?t) |- _ ] => eapply Tr_EPath in H;[|cbn;reflexivity]; destructH' H; cbn_nl' H
+  | [ H : Tr ?t |- _ ] => destruct (ne_front t) as [[p i] s] eqn:Q;
+                        eapply Tr_EPath in H;[clear Q|apply Q]; destructH' H; cbn_nl' H
   end.
 
 Ltac spot_path_t :=
   try spot_path_e;
   lazymatch goal with
-  | [ H : EPath _ _ _ |- _ ] => eapply EPath_TPath in H; cbn in H
+  | [ H : EPath _ _ _ |- _ ] => eapply EPath_TPath in H; cbn_nl' H
   end.
 
 Ltac spot_path_c :=
   try spot_path_t;
   lazymatch goal with
-    [ H : TPath _ _ _ |- _ ] => eapply TPath_CPath in H; cbn in H
+    [ H : TPath _ _ _ |- _ ] => eapply TPath_CPath in H; cbn_nl' H
   end.
 
 Ltac spot_path :=
   lazymatch goal with
+  | [ H : CPath' _ |- _ ] => unfold CPath' in H;spot_path
+  | [ H : TPath' _ |- _ ] => unfold TPath' in H;spot_path
+  | [ H : EPath' _ |- _ ] => unfold EPath' in H;spot_path
+  | [ |- CPath' _ ] => repeat spot_path_c; eapply cpath_cpath';eauto
+  | [ |- TPath' _ ] => repeat spot_path_t; eapply tpath_tpath';eauto
+  | [ |- EPath' _ ] => repeat spot_path_e; eapply epath_epath';eauto
   | [ |- CPath _ _ _ ] => repeat (spot_path_c;eauto)
   | [ |- TPath _ _ _ ] => repeat (spot_path_t;eauto)
   | [ |- EPath _ _ _ ] => repeat (spot_path_e;eauto)
